# **Task 1**
Editied by Pinheng Chen, z5383372.  
Last Edited time: 2023/06/05
## Question:
![Task1](/Tasks/task-imgs/task1.png)
## Solution:
Given $m=_{(n)}m'$ and $p_{(n)}p'$,  
we know $n\mid (m-m')$ and $n\mid (p-p')$,  
so $\exists k_1, k_2\in \mathbb{Z}$, $k_1n=(m-m')$ and $k_2n=(p-p')$,  
let $k_1n + k_2n = (m-m') + (p-p')$,  
then $(k_1+k_2)n = (m+p) - (m'+ p')\cdots\cdots Equation1$.  
Obviously, $Equation1$ exactly refers to $n\mid ((m+p) - (m' + p'))$,  
hence, $m+p=_{(n)}m'+p'$ is correct.
